spec/sail/lean/Out.lean
@@ -27,7 +27,7 @@ open CompareOp
 open BranchRegisterExecutionTarget
 open BarrierExecutionTarget
 
-/-- Type quantifiers: k_ex24101_ : Bool, k_ex24100_ : Bool -/
+/-- Type quantifiers: k_ex24655_ : Bool, k_ex24654_ : Bool -/
 def neq_bool (x : Bool) (y : Bool) : Bool :=
   (! (x == y))
 
@@ -177,7 +177,7 @@ def ConditionHolds (cond : (BitVec 4)) (nzcv : (BitVec 4)) : Bool :=
   then (! result)
   else result
 
-/-- Type quantifiers: k_ex24285_ : Bool, k_ex24284_ : Bool, k_datasize : Nat, k_datasize ∈
+/-- Type quantifiers: k_ex24839_ : Bool, k_ex24838_ : Bool, k_datasize : Nat, k_datasize ∈
   {32, 64} -/
 def integer_conditional_select (condition : (BitVec 4)) (nzcv : (BitVec 4)) (else_inc : Bool) (else_inv : Bool) (operand1 : (BitVec k_datasize)) (operand2 : (BitVec k_datasize)) : (BitVec k_datasize) :=
   let result : (BitVec k_datasize) := operand2
@@ -193,7 +193,7 @@ def integer_conditional_select (condition : (BitVec 4)) (nzcv : (BitVec 4)) (els
     then (BitVec.addInt result 1)
     else result)
 
-/-- Type quantifiers: k_ex24301_ : Bool, k_datasize : Nat, k_datasize ∈ {32, 64} -/
+/-- Type quantifiers: k_ex24855_ : Bool, k_datasize : Nat, k_datasize ∈ {32, 64} -/
 def integer_conditional_compare_register (condition : (BitVec 4)) (nzcv : (BitVec 4)) (flags__arg : (BitVec 4)) (operand1 : (BitVec k_datasize)) (operand2__arg : (BitVec k_datasize)) (sub_op : Bool) : (BitVec 4) :=
   let flags : (BitVec 4) := flags__arg
   let operand2 : (BitVec k_datasize) := operand2__arg
@@ -338,7 +338,7 @@ def vector_transfer_integer_dup (datasize : Nat) (elements : Nat) (esize : Nat) 
     loop_vars := (aset_Elem result e esize element)
   (pure loop_vars)
 
-/-- Type quantifiers: k_ex24440_ : Bool, datasize : Nat, elements : Nat, esize : Nat, esize ≥ 1
+/-- Type quantifiers: k_ex24994_ : Bool, datasize : Nat, elements : Nat, esize : Nat, esize ≥ 1
   ∧ elements ≥ 1 ∧ (elements * esize) = datasize -/
 def vector_arithmetic_binary_uniform_add_wrapping_single (datasize : Nat) (elements : Nat) (esize : Nat) (operand1 : (BitVec datasize)) (operand2 : (BitVec datasize)) (sub_op : Bool) : (BitVec datasize) := Id.run do
   let result : (BitVec datasize) := (Zeros datasize)
@@ -361,7 +361,7 @@ def vector_arithmetic_binary_uniform_add_wrapping_single (datasize : Nat) (eleme
     (pure loop_vars) ) : Id ((BitVec esize) × (BitVec esize) × (BitVec datasize)) )
   (pure result)
 
-/-- Type quantifiers: k_ex24508_ : Bool, k_ex24507_ : Bool, datasize : Nat, elements : Nat, esize :
+/-- Type quantifiers: k_ex25062_ : Bool, k_ex25061_ : Bool, datasize : Nat, elements : Nat, esize :
   Nat, esize ≥ 1 ∧ elements ≥ 1 ∧ (elements * esize) = datasize -/
 def vector_arithmetic_binary_uniform_maxmin_single (datasize : Nat) (elements : Nat) (esize : Nat) (operand1 : (BitVec datasize)) (operand2 : (BitVec datasize)) (minimum : Bool) (is_unsigned : Bool) : (BitVec datasize) := Id.run do
   let result : (BitVec datasize) := (Zeros datasize)
@@ -386,7 +386,7 @@ def vector_arithmetic_binary_uniform_maxmin_single (datasize : Nat) (elements : 
     (pure loop_vars) ) : Id (Int × Int × Int × (BitVec datasize)) )
   (pure result)
 
-/-- Type quantifiers: k_ex24559_ : Bool, k_ex24558_ : Bool, datasize : Nat, elements : Nat, esize :
+/-- Type quantifiers: k_ex25113_ : Bool, k_ex25112_ : Bool, datasize : Nat, elements : Nat, esize :
   Nat, esize ≥ 1 ∧ elements ≥ 1 ∧ (elements * esize) = datasize -/
 def vector_arithmetic_binary_uniform_cmp_int (cmp_eq : Bool) (datasize : Nat) (elements : Nat) (esize : Nat) (operand1 : (BitVec datasize)) (operand2 : (BitVec datasize)) (is_unsigned : Bool) : (BitVec datasize) := Id.run do
   let result : (BitVec datasize) := (Zeros datasize)
@@ -415,7 +415,7 @@ def vector_arithmetic_binary_uniform_cmp_int (cmp_eq : Bool) (datasize : Nat) (e
     (pure loop_vars) ) : Id (Int × Int × (BitVec datasize) × Bool) )
   (pure result)
 
-/-- Type quantifiers: k_ex24605_ : Bool, datasize : Nat, elements : Nat, esize : Nat, esize ≥ 1
+/-- Type quantifiers: k_ex25159_ : Bool, datasize : Nat, elements : Nat, esize : Nat, esize ≥ 1
   ∧ elements ≥ 1 ∧ (elements * esize) = datasize -/
 def vector_arithmetic_binary_uniform_cmp_bitwise (and_test : Bool) (datasize : Nat) (elements : Nat) (esize : Nat) (operand1 : (BitVec datasize)) (operand2 : (BitVec datasize)) : (BitVec datasize) := Id.run do
   let result : (BitVec datasize) := (Zeros datasize)
@@ -494,7 +494,7 @@ def vector_arithmetic_unary_cmp_int_bulk (comparison : CompareOp) (datasize : Na
     (pure loop_vars) ) : Id (Int × (BitVec datasize) × Bool) )
   (pure result)
 
-/-- Type quantifiers: k_ex24734_ : Bool, datasize : Nat, elements : Nat, esize : Nat, esize ≥ 1
+/-- Type quantifiers: k_ex25288_ : Bool, datasize : Nat, elements : Nat, esize : Nat, esize ≥ 1
   ∧ elements ≥ 1 ∧ (elements * esize) = datasize -/
 def vector_arithmetic_binary_uniform_sub_saturating (datasize : Nat) (elements : Nat) (esize : Nat) (operand1 : (BitVec datasize)) (operand2 : (BitVec datasize)) (is_unsigned : Bool) : (BitVec datasize) := Id.run do
   let result : (BitVec datasize) := (Zeros datasize)
@@ -517,7 +517,7 @@ def vector_arithmetic_binary_uniform_sub_saturating (datasize : Nat) (elements :
     (pure loop_vars) ) : Id (Int × Int × Int × (BitVec datasize)) )
   (pure result)
 
-/-- Type quantifiers: k_ex24785_ : Bool, shift : Int, k_ex24783_ : Bool, k_ex24782_ : Bool, datasize
+/-- Type quantifiers: k_ex25339_ : Bool, shift : Int, k_ex25337_ : Bool, k_ex25336_ : Bool, datasize
   : Nat, elements : Nat, esize : Nat, esize ≥ 1 ∧
   elements ≥ 1 ∧ (elements * esize) = datasize -/
 def vector_shift_right (accumulate : Bool) (datasize : Nat) (elements : Nat) (esize : Nat) (operand : (BitVec datasize)) (accumulator : (BitVec datasize)) (round : Bool) (shift : Int) (is_unsigned : Bool) : (BitVec datasize) := Id.run do
@@ -547,7 +547,7 @@ def vector_shift_right (accumulate : Bool) (datasize : Nat) (elements : Nat) (es
     (pure loop_vars) ) : Id (Int × (BitVec datasize)) )
   (pure result)
 
-/-- Type quantifiers: k_ex24838_ : Bool, datasize : Nat, elements : Nat, elements ≥ 1 ∧
+/-- Type quantifiers: k_ex25392_ : Bool, datasize : Nat, elements : Nat, elements ≥ 1 ∧
   (elements * 8) = datasize ∧ datasize ≤ 128 -/
 def vector_transfer_vector_table (datasize : Nat) (elements : Nat) (is_tbl : Bool) (indices : (BitVec datasize)) (table : (BitVec 128)) (dst : (BitVec datasize)) : (BitVec datasize) := Id.run do
   let result : (BitVec datasize) :=
@@ -571,7 +571,7 @@ def vector_transfer_vector_extract (datasize : Nat) (hi : (BitVec datasize)) (lo
   let concat : (BitVec (2 * datasize)) := (hi +++ lo)
   (BitVec.slice concat position datasize)
 
-/-- Type quantifiers: k_ex24870_ : Bool, k_ex24869_ : Bool, datasize : Nat, elements : Nat, esize :
+/-- Type quantifiers: k_ex25424_ : Bool, k_ex25423_ : Bool, datasize : Nat, elements : Nat, esize :
   Nat, esize ≥ 1 ∧ elements ≥ 1 ∧ (elements * esize) = datasize -/
 def vector_reduce_intmax (datasize : Nat) (elements : Nat) (esize : Nat) (operand : (BitVec datasize)) (min : Bool) (is_unsigned : Bool) : (BitVec esize) := Id.run do
   let maxmin : Int := 0
@@ -627,7 +627,7 @@ def num_of_LogicalOp (arg_ : LogicalOp) : Int :=
   | .LogicalOp_EOR => 1
   | .LogicalOp_ORR => 2
 
-/-- Type quantifiers: k_ex24928_ : Bool, datasize : Nat, datasize ≥ 1 -/
+/-- Type quantifiers: k_ex25482_ : Bool, datasize : Nat, datasize ≥ 1 -/
 def vector_arithmetic_binary_uniform_logical_andorr (datasize : Nat) (invert : Bool) (operand1 : (BitVec datasize)) (operand2__arg : (BitVec datasize)) (op : LogicalOp) : (BitVec datasize) :=
   let operand2 : (BitVec datasize) := operand2__arg
   let result : (BitVec datasize) := (Zeros datasize)
@@ -700,7 +700,7 @@ def FPNeg (op : (BitVec k_N)) : (BitVec k_N) :=
 def FPAbs (op : (BitVec k_N)) : (BitVec k_N) :=
   (0#1 +++ (BitVec.slice op 0 ((Sail.BitVec.length op) -i 1)))
 
-/-- Type quantifiers: k_ex25087_ : Bool, datasize : Nat, elements : Nat, esize : Nat, esize ∈
+/-- Type quantifiers: k_ex25641_ : Bool, datasize : Nat, elements : Nat, esize : Nat, esize ∈
   {32, 64} ∧ elements ≥ 1 ∧ (elements * esize) = datasize -/
 def vector_arithmetic_binary_uniform_add_fp (datasize : Nat) (elements : Nat) (esize : Nat) (operand1 : (BitVec datasize)) (operand2 : (BitVec datasize)) (fpcr : (BitVec 32)) (pair : Bool) : (BitVec datasize) := Id.run do
   let result : (BitVec datasize) := (Zeros datasize)
@@ -730,7 +730,7 @@ def vector_arithmetic_binary_uniform_add_fp (datasize : Nat) (elements : Nat) (e
     (pure loop_vars) ) : Id ((BitVec esize) × (BitVec esize) × (BitVec datasize)) )
   (pure result)
 
-/-- Type quantifiers: k_ex25194_ : Bool, datasize : Nat, elements : Nat, esize : Nat, esize ∈
+/-- Type quantifiers: k_ex25748_ : Bool, datasize : Nat, elements : Nat, esize : Nat, esize ∈
   {32, 64} ∧ elements ≥ 1 ∧ (elements * esize) = datasize -/
 def vector_arithmetic_binary_uniform_sub_fp (datasize : Nat) (elements : Nat) (esize : Nat) (operand1 : (BitVec datasize)) (operand2 : (BitVec datasize)) (fpcr : (BitVec 32)) (abs : Bool) : (BitVec datasize) := Id.run do
   let result : (BitVec datasize) := (Zeros datasize)
@@ -778,7 +778,7 @@ def vector_arithmetic_binary_uniform_mul_fp_product (datasize : Nat) (elements :
     (pure loop_vars) ) : Id ((BitVec esize) × (BitVec esize) × (BitVec datasize)) )
   (pure result)
 
-/-- Type quantifiers: k_ex25368_ : Bool, datasize : Nat, elements : Nat, esize : Nat, esize ∈
+/-- Type quantifiers: k_ex25922_ : Bool, datasize : Nat, elements : Nat, esize : Nat, esize ∈
   {32, 64} ∧ elements ≥ 1 ∧ (elements * esize) = datasize -/
 def vector_arithmetic_binary_uniform_mul_fp_fused (datasize : Nat) (elements : Nat) (esize : Nat) (operand1 : (BitVec datasize)) (operand2 : (BitVec datasize)) (operand3 : (BitVec datasize)) (fpcr : (BitVec 32)) (sub_op : Bool) : (BitVec datasize) := Id.run do
   let result : (BitVec datasize) := (Zeros datasize)
@@ -804,7 +804,7 @@ def vector_arithmetic_binary_uniform_mul_fp_fused (datasize : Nat) (elements : N
     (pure loop_vars) ) : Id ((BitVec esize) × (BitVec esize) × (BitVec datasize)) )
   (pure result)
 
-/-- Type quantifiers: k_ex25444_ : Bool, k_ex25443_ : Bool, datasize : Nat, elements : Nat, esize :
+/-- Type quantifiers: k_ex25998_ : Bool, k_ex25997_ : Bool, datasize : Nat, elements : Nat, esize :
   Nat, esize ∈ {32, 64} ∧ elements ≥ 1 ∧ (elements * esize) = datasize -/
 def vector_arithmetic_binary_uniform_maxmin_fp_1985 (datasize : Nat) (elements : Nat) (esize : Nat) (operand1 : (BitVec datasize)) (operand2 : (BitVec datasize)) (fpcr : (BitVec 32)) (minimum : Bool) (pair : Bool) : (BitVec datasize) := Id.run do
   let result : (BitVec datasize) := (Zeros datasize)
@@ -836,7 +836,7 @@ def vector_arithmetic_binary_uniform_maxmin_fp_1985 (datasize : Nat) (elements :
     (pure loop_vars) ) : Id ((BitVec esize) × (BitVec esize) × (BitVec datasize)) )
   (pure result)
 
-/-- Type quantifiers: k_ex25542_ : Bool, k_ex25541_ : Bool, datasize : Nat, elements : Nat, esize :
+/-- Type quantifiers: k_ex26096_ : Bool, k_ex26095_ : Bool, datasize : Nat, elements : Nat, esize :
   Nat, esize ∈ {32, 64} ∧ elements ≥ 1 ∧ (elements * esize) = datasize -/
 def vector_arithmetic_binary_uniform_maxmin_fp_2008 (datasize : Nat) (elements : Nat) (esize : Nat) (operand1 : (BitVec datasize)) (operand2 : (BitVec datasize)) (fpcr : (BitVec 32)) (minimum : Bool) (pair : Bool) : (BitVec datasize) := Id.run do
   let result : (BitVec datasize) := (Zeros datasize)
@@ -886,7 +886,7 @@ def vector_arithmetic_unary_special_sqrt (datasize : Nat) (elements : Nat) (esiz
     (pure loop_vars) ) : Id ((BitVec esize) × (BitVec datasize)) )
   (pure result)
 
-/-- Type quantifiers: k_ex25689_ : Bool, datasize : Nat, elements : Nat, esize : Nat, esize ∈
+/-- Type quantifiers: k_ex26243_ : Bool, datasize : Nat, elements : Nat, esize : Nat, esize ∈
   {32, 64} ∧ elements ≥ 1 ∧ (elements * esize) = datasize -/
 def vector_arithmetic_unary_diffneg_fp (datasize : Nat) (elements : Nat) (esize : Nat) (operand : (BitVec datasize)) (neg : Bool) : (BitVec datasize) := Id.run do
   let result : (BitVec datasize) := (Zeros datasize)
@@ -907,6 +907,26 @@ def vector_arithmetic_unary_diffneg_fp (datasize : Nat) (elements : Nat) (esize 
         (element, result)
     (pure loop_vars) ) : Id ((BitVec esize) × (BitVec datasize)) )
   (pure result)
+
+def decode64_str64_unsigned_pure (op_code : (BitVec 32)) : (Bool × (BitVec 5) × (BitVec 5) × (BitVec 12)) :=
+  let Rt : (BitVec 5) := (BitVec.slice op_code 0 5)
+  let Rn : (BitVec 5) := (BitVec.slice op_code 5 5)
+  let imm12 : (BitVec 12) := (BitVec.slice op_code 10 12)
+  if (((op_code &&& 0xFFC00000#32) == 0xF9000000#32) : Bool)
+  then (true, Rt, Rn, imm12)
+  else (false, Rt, Rn, imm12)
+
+def str64_unsigned_store_request_pure (Rt : (BitVec 5)) (Rn : (BitVec 5)) (imm12 : (BitVec 12)) (rn_value : (BitVec 64)) (rt_value : (BitVec 64)) (sp_value : (BitVec 64)) : ((BitVec 64) × (BitVec 64)) :=
+  let base : (BitVec 64) :=
+    if ((Rn == 0b11111#5) : Bool)
+    then sp_value
+    else rn_value
+  let data : (BitVec 64) :=
+    if ((Rt == 0b11111#5) : Bool)
+    then (Zeros 64)
+    else rt_value
+  let offset : (BitVec 64) := ((Sail.BitVec.zeroExtend imm12 64) <<< 3)
+  ((base + offset), data)
 
 def undefined_MemBarrierOp (_ : Unit) : SailM MemBarrierOp := do
   (internal_pick
@@ -1176,7 +1196,7 @@ def undefined_PlainERETDecode (_ : Unit) : SailM PlainERETDecode := do
           pac := ← (undefined_bool ())
           use_key_a := ← (undefined_bool ()) })
 
-/-- Type quantifiers: k_ex25983_ : Bool -/
+/-- Type quantifiers: k_ex26609_ : Bool -/
 def decode64_plain_eret_pure (op_code : (BitVec 32)) (at_el0 : Bool) : PlainERETDecode :=
   let op4 : (BitVec 5) := (BitVec.slice op_code 0 5)
   let Rn : (BitVec 5) := (BitVec.slice op_code 5 5)
@@ -1252,8 +1272,8 @@ def decode64_system_write_vttbr_el2_pure (op_code : (BitVec 32)) : (Bool × Syst
   then (system_register_vttbr_el2_target_pure o0 op1 CRn CRm op2 Rt)
   else (false, SystemRegisterWriteTarget_VTTBR_EL2, Rt)
 
-/-- Type quantifiers: k_ex26682_ : Bool, k_ex26681_ : Bool, k_ex26680_ : Bool, k_ex26679_ : Bool, k_ex26678_
-  : Bool, k_ex26677_ : Bool -/
+/-- Type quantifiers: k_ex27308_ : Bool, k_ex27307_ : Bool, k_ex27306_ : Bool, k_ex27305_ : Bool, k_ex27304_
+  : Bool, k_ex27303_ : Bool -/
 def aarch64_sysregwrite_vttbr_el2_pure (at_el1 : Bool) (hcr_nv : Bool) (hcr_nv2 : Bool) (hcr_tge : Bool) (scr_ns : Bool) (scr_eel2 : Bool) (old_value : (BitVec 64)) (val_name : (BitVec 64)) : (Bool × (BitVec 64)) :=
   let redirected : Bool :=
     (at_el1 && (hcr_nv && (hcr_nv2 && ((! hcr_tge) && (scr_ns || scr_eel2)))))
@@ -1277,8 +1297,8 @@ def decode64_system_write_vtcr_el2_pure (op_code : (BitVec 32)) : (Bool × Syste
   then (system_register_vtcr_el2_target_pure o0 op1 CRn CRm op2 Rt)
   else (false, SystemRegisterWriteTarget_VTCR_EL2, Rt)
 
-/-- Type quantifiers: k_ex26804_ : Bool, k_ex26803_ : Bool, k_ex26802_ : Bool, k_ex26801_ : Bool, k_ex26800_
-  : Bool, k_ex26799_ : Bool -/
+/-- Type quantifiers: k_ex27430_ : Bool, k_ex27429_ : Bool, k_ex27428_ : Bool, k_ex27427_ : Bool, k_ex27426_
+  : Bool, k_ex27425_ : Bool -/
 def aarch64_sysregwrite_vtcr_el2_pure (at_el1 : Bool) (hcr_nv : Bool) (hcr_nv2 : Bool) (hcr_tge : Bool) (scr_ns : Bool) (scr_eel2 : Bool) (old_value : (BitVec 32)) (val_name : (BitVec 64)) : (Bool × (BitVec 32)) :=
   let redirected : Bool :=
     (at_el1 && (hcr_nv && (hcr_nv2 && ((! hcr_tge) && (scr_ns || scr_eel2)))))
@@ -1321,8 +1341,8 @@ def decode64_system_write_cntvoff_el2_pure (op_code : (BitVec 32)) : (Bool × Sy
   then (system_register_cntvoff_el2_target_pure o0 op1 CRn CRm op2 Rt)
   else (false, SystemRegisterWriteTarget_CNTVOFF_EL2, Rt)
 
-/-- Type quantifiers: k_ex27040_ : Bool, k_ex27039_ : Bool, k_ex27038_ : Bool, k_ex27037_ : Bool, k_ex27036_
-  : Bool, k_ex27035_ : Bool -/
+/-- Type quantifiers: k_ex27666_ : Bool, k_ex27665_ : Bool, k_ex27664_ : Bool, k_ex27663_ : Bool, k_ex27662_
+  : Bool, k_ex27661_ : Bool -/
 def aarch64_sysregwrite_cntvoff_el2_pure (at_el1 : Bool) (hcr_nv : Bool) (hcr_nv2 : Bool) (hcr_tge : Bool) (scr_ns : Bool) (scr_eel2 : Bool) (old_value : (BitVec 64)) (val_name : (BitVec 64)) : (Bool × (BitVec 64)) :=
   let redirected : Bool :=
     (at_el1 && (hcr_nv && (hcr_nv2 && ((! hcr_tge) && (scr_ns || scr_eel2)))))
@@ -1346,8 +1366,8 @@ def decode64_system_write_sp_el1_pure (op_code : (BitVec 32)) : (Bool × SystemR
   then (system_register_sp_el1_target_pure o0 op1 CRn CRm op2 Rt)
   else (false, SystemRegisterWriteTarget_SP_EL1, Rt)
 
-/-- Type quantifiers: k_ex27162_ : Bool, k_ex27161_ : Bool, k_ex27160_ : Bool, k_ex27159_ : Bool, k_ex27158_
-  : Bool, k_ex27157_ : Bool -/
+/-- Type quantifiers: k_ex27788_ : Bool, k_ex27787_ : Bool, k_ex27786_ : Bool, k_ex27785_ : Bool, k_ex27784_
+  : Bool, k_ex27783_ : Bool -/
 def aarch64_sysregwrite_sp_el1_pure (at_el1 : Bool) (hcr_nv : Bool) (hcr_nv2 : Bool) (hcr_tge : Bool) (scr_ns : Bool) (scr_eel2 : Bool) (old_value : (BitVec 64)) (val_name : (BitVec 64)) : (Bool × (BitVec 64)) :=
   let redirected : Bool :=
     (at_el1 && (hcr_nv && (hcr_nv2 && ((! hcr_tge) && (scr_ns || scr_eel2)))))
@@ -1409,8 +1429,8 @@ def decode64_system_write_hcr_el2_pure (op_code : (BitVec 32)) : (Bool × System
   then (system_register_hcr_el2_target_pure o0 op1 CRn CRm op2 Rt)
   else (false, SystemRegisterWriteTarget_HCR_EL2, Rt)
 
-/-- Type quantifiers: k_ex27512_ : Bool, k_ex27511_ : Bool, k_ex27510_ : Bool, k_ex27509_ : Bool, k_ex27508_
-  : Bool, k_ex27507_ : Bool -/
+/-- Type quantifiers: k_ex28138_ : Bool, k_ex28137_ : Bool, k_ex28136_ : Bool, k_ex28135_ : Bool, k_ex28134_
+  : Bool, k_ex28133_ : Bool -/
 def aarch64_sysregwrite_hcr_el2_pure (at_el1 : Bool) (old_hcr_nv : Bool) (old_hcr_nv2 : Bool) (old_hcr_tge : Bool) (scr_ns : Bool) (scr_eel2 : Bool) (old_value : (BitVec 64)) (val_name : (BitVec 64)) : (Bool × (BitVec 64)) :=
   let redirected : Bool :=
     (at_el1 && (old_hcr_nv && (old_hcr_nv2 && ((! old_hcr_tge) && (scr_ns || scr_eel2)))))
@@ -1449,7 +1469,7 @@ def undefined_ColdEntryRegisterSequenceResult (_ : Unit) : SailM ColdEntryRegist
           write6 := ← (undefined_SystemRegisterWriteTarget ())
           write7 := ← (undefined_SystemRegisterWriteTarget ()) })
 
-/-- Type quantifiers: k_ex27534_ : Bool, k_ex27533_ : Bool, k_ex27532_ : Bool, k_ex27531_ : Bool -/
+/-- Type quantifiers: k_ex28160_ : Bool, k_ex28159_ : Bool, k_ex28158_ : Bool, k_ex28157_ : Bool -/
 def eret_nv_trap_route_pure (have_nv_ext : Bool) (el2_enabled : Bool) (at_el1 : Bool) (hcr_nv : Bool) : Bool :=
   (((have_nv_ext && el2_enabled) && at_el1) && hcr_nv)
 
@@ -1458,14 +1478,14 @@ def undefined_PlainERETInputsAtEL2 (_ : Unit) : SailM PlainERETInputsAtEL2 := do
           target := ← (undefined_bitvector 64)
           spsr := ← (undefined_bitvector 32) })
 
-/-- Type quantifiers: k_ex27538_ : Bool, k_ex27537_ : Bool -/
+/-- Type quantifiers: k_ex28164_ : Bool, k_ex28163_ : Bool -/
 def aarch64_plain_eret_at_el2_inputs_pure (have_nv_ext : Bool) (el2_enabled : Bool) (state : ColdEntryRegisterState) : PlainERETInputsAtEL2 :=
   let hcr_nv : Bool := ((BitVec.access state.hcr_el2 42) == 1#1)
   { dedicated_nv_trap := (eret_nv_trap_route_pure have_nv_ext el2_enabled false hcr_nv)
     target := state.elr_el2
     spsr := state.spsr_el2 }
 
-/-- Type quantifiers: k_ex27542_ : Bool, k_ex27541_ : Bool -/
+/-- Type quantifiers: k_ex28168_ : Bool, k_ex28167_ : Bool -/
 def aarch64_cold_entry_register_sequence_at_el2_pure (old_state : ColdEntryRegisterState) (inputs : ColdEntryRegisterInputs) (scr_ns : Bool) (scr_eel2 : Bool) : ColdEntryRegisterSequenceResult :=
   let old_hcr_nv : Bool := ((BitVec.access old_state.hcr_el2 42) == 1#1)
   let old_hcr_nv2 : Bool := ((BitVec.access old_state.hcr_el2 45) == 1#1)
